Theorem8.v
@@ -1,0 +1,23 @@
+Require Import case_coq.
+Require Import List.
+Require Import Coq.Sets.Constructive_sets.
+Require Import Coq.Arith.EqNat.
+Require Import Coq.Relations.Relation_Definitions.
+Require Import Coq.Relations.Relation_Operators.
+Require Import Coq.Arith.Compare_dec.
+Require Import Coq.Program.Tactics.
+Require Import parametes_coq.
+Require Import config_coq.
+Import Config.
+Require Import oper_semantic_coq.
+Require Import axioms_coq.
+Require Import theorems_coq.
+Require Import contract_definition.
+Require Import contract_subs.
+Require Import contract_Eval.
+Require Import lemma5.
+Require Import Theorem7.
+Import parameters.
+Import Operational_Semantics.
+
+Theorem Theorem8: forall (Ex Ex':Exec) (θ θ:Store), WF Ex -> CausCons θ Ex -> 
